Add CF tactics for raise and handle, and corresponding examples

characteristic/cfComputeLib.sml
@@ -23,7 +23,6 @@ val add_cf_aux_compset = computeLib.extend_compset
      cfTheory.pat_typechecks_def,
      cfTheory.pat_without_Pref_def,
      cfTheory.validate_pat_def,
-     cfTheory.build_cases_def,
      cfNormalizeTheory.exp2v_def,
      cfNormalizeTheory.exp2v_list_def,
      cfNormalizeTheory.dest_opapp_def
