characteristic/cfTacticsLib.sig
@@ -109,6 +109,28 @@ sig
   *)
   val xffi : tactic
 
+  (* [xraise] applies on characteristic formulae for raise, of the form
+     [cf_raise ..].
+  *)
+  val xraise : tactic
+
+  (* [xhandle] applies on characteristic formulae for exception handling,
+     of the form [cf_handle ..].
+
+     A post-condition for the evaluation of the body must be provided.
+  *)
+  val xhandle : term quotation -> tactic
+
+  (* [xcases] is somewhat similar to [xmatch]. It applies to characteristic
+     formalue of the form [cf_cases ...], and simplifies them. Such formulae are
+     typically produced by [xhandle].
+
+     [xcases] is not automatically called by [xhandle] as the user is expected
+     to pull facts using [xpull], perform case analysis, unfold representation
+     predicates, ..., before calling [xcases].
+  *)
+  val xcases : tactic
+
   (* low level / debugging *)
   val xlocal : tactic
   val xapply : thm -> tactic
